Cleaned Wellformedness.v

Wellformedness.v
@@ -1,269 +1,295 @@
+(* Celsius project *)
+(* Clément Blaudeau - Lamp@EPFL 2021 *)
+(** This file defines the notion of wellformedness for scopes. The set of reachable locations must all be valid locations of the store - that is, locations that are inside of the store. The main result is to show that if we start from a wellformed store that contains the local environment ρ and the [this] pointer, then we end up with a wellformed store that contains the location of the result *)
+
 From Celsius Require Export Trees Eval PartialMonotonicity Reachability Compatibility.
-Require Import ssreflect ssrbool Psatz List.
+Require Import ssreflect ssrbool Psatz List Sets.Ensembles Coq.Program.Tactics.
 Import ListNotations.
 Open Scope nat_scope.
-Require Import Sets.Ensembles.
 
-Create HintDb wf.
+Hint Resolve Union_intror: wf.
+Hint Resolve Union_introl: wf.
+Hint Resolve In_singleton: wf.
 
-Definition wf σ := forall l C ω, getObj σ l = Some(C,ω) -> forall f l, getVal ω f = Some l -> l < dom σ.
+(** ** Definitions and notations *)
+(** A wellformed store only contains pointers to locations that are within itself *)
+Definition wf σ :=
+  forall l C ω,
+    getObj σ l = Some(C,ω) ->
+    forall f l,
+      getVal ω f = Some l ->
+      l < dom σ. (**r [l ∈ dom σ] *)
 
-Definition storeSubset (σ: Store) L := (forall l, (l ∈ L) -> l < (dom σ)).
+(** A set of locations is contained in a store: [L ⪽ σ] *)
+Definition storeSubset (σ: Store) L :=
+  forall l, l ∈ L ->
+       l < dom σ.
+
+(** The codomain of an environment is the set of locations it contains *)
+Definition codom (ρ: Env) : (LocSet) :=
+  fun l => (List.In l ρ).
+
 Notation "L ⪽ σ" := (storeSubset σ L) (at level 80).
-Definition codom (ρ: Env) : (LocSet):=
-  fun (l: Loc) => (List.In l ρ).
+Notation " a ∪ { b } " := (Union Loc a (Singleton Loc b)) (at level 80).
 
+(** ** Basic results *)
 
-
-Lemma storeSubset_trans : forall a s s', dom s <= dom s' -> a ⪽ s -> a ⪽ s'.
+Lemma storeSubset_trans :
+  forall a s s',
+    dom s <= dom s' ->
+    a ⪽ s ->
+    a ⪽ s'.
 Proof.
-  intros. intros l Hl.
-  pose proof (H0 l Hl).
-  lia.
+  unfold storeSubset; steps.
+  eapply H0 in H1 ; lia.
 Qed.
-Hint Resolve storeSubset_trans: wf.
 
-Lemma storeSubset_union : forall a b s, a ⪽ s -> b ⪽ s -> (a∪b) ⪽ s.
+Lemma storeSubset_union :
+  forall a b s,
+    a ⪽ s ->
+    b ⪽ s ->
+    (a∪b) ⪽ s.
 Proof.
   unfold storeSubset; intros.
   induction H1; eauto.
 Qed.
-Hint Resolve storeSubset_union: wf.
 
-Lemma storeSubset_union_l : forall a b s, (a∪b) ⪽ s -> a ⪽ s.
+Lemma storeSubset_union_l :
+  forall a b s,
+    (a∪b) ⪽ s -> a ⪽ s.
 Proof.
-  unfold storeSubset; intros.
-  apply H. eauto using Union_introl.
+  unfold storeSubset; eauto with wf.
 Qed.
-Hint Resolve storeSubset_union_l: wf.
 
-Lemma storeSubset_union_r : forall a b s, (a∪b) ⪽ s -> b ⪽ s.
+Lemma storeSubset_union_r :
+  forall a b s,
+    (a∪b) ⪽ s -> b ⪽ s.
 Proof.
-  unfold storeSubset; intros.
-  apply H. eauto using Union_intror.
+  unfold storeSubset; eauto with wf.
 Qed.
-Hint Resolve storeSubset_union_r: wf.
 
-Lemma storeSubset_add : forall v a s,
+Lemma storeSubset_add :
+  forall v a s,
     codom (v :: a) ⪽ s <-> v < dom s /\ codom a ⪽ s.
 Proof.
-  split; intros.
-  + unfold storeSubset in H.
-    split. apply H.
-    unfold codom, List.In, In; left => //.
-    intros l Hl. apply H.
-    unfold codom, List.In, In; right => //.
-  + intros l Hl. unfold codom, List.In, In in Hl. move: Hl=> [Hl|Hl]; steps.
+  unfold codom, List.In, In, storeSubset in *; split.
+  + steps; eapply_any; steps; right => //.
+  + steps; move: H0 => [Hl|Hl]; steps.
 Qed.
-Hint Resolve storeSubset_add: wf.
 
-Notation " a ∪ { b } " := (Union Loc a (Singleton Loc b)) (at level 80).
-Lemma storeSubset_singleton : forall a b σ, a ∪ {b} ⪽ σ -> b < dom σ.
+Lemma storeSubset_singleton :
+  forall a b σ,
+    a ∪ {b} ⪽ σ -> b < dom σ.
 Proof.
-  intros. apply (H b).
-  eauto using Union_intror, In_singleton.
+  intros.
+  eapply_any; eauto with wf.
 Qed.
-Hint Resolve storeSubset_singleton: wf.
 
-Lemma storeSubset_singleton2 : forall a σ, (Singleton Loc a) ⪽ σ <-> a < dom σ.
+Lemma storeSubset_singleton2 :
+  forall a σ,
+    (Singleton Loc a) ⪽ σ <-> a < dom σ.
 Proof.
   unfold storeSubset; steps;
     [induction (H a) | induction H0] ; steps.
 Qed.
-Hint Resolve storeSubset_singleton2: wf.
 
 Lemma storeSubset_codom_empty : forall s, codom [] ⪽ s.
 Proof.
-  intros s l Hl.
-  steps.
+  unfold storeSubset; steps.
 Qed.
-Hint Resolve storeSubset_codom_empty: wf.
 
 Lemma codom_empty_union: forall a, (codom [] ∪ a) = a.
 Proof.
   intros.
   apply Extensionality_Ensembles.
-  unfold Same_set. unfold Included; repeat steps || destruct H.
-  eapply Union_intror => //.
+  unfold Same_set, Included;
+    repeat steps || destruct H;
+    eauto with wf.
 Qed.
 
-
+(** In preparation for initialization theorems, we have technical results about adding a location *)
 Lemma wf_add : forall s c ρ, wf s -> codom ρ ⪽ s -> wf (s ++ [(c,ρ)]).
 Proof.
   unfold wf, dom; intros.
-  pose proof (getObj_dom _ _ _ H1).
-  pose proof (PeanoNat.Nat.eq_dec l (length s)) as [Hl0 | Hl0].
-  + rewrite app_length. simpl. subst.
-    rewrite getObj_last in H1. invert_constructor_equalities; subst.
-    rewrite PeanoNat.Nat.add_1_r. apply (PeanoNat.Nat.lt_trans _ (length s) _); try lia.
-    apply H0.
-    unfold getVal in H2. apply nth_error_In in H2. eauto.
-  + unfold dom in *. rewrite_anywhere app_length. simpl in H2.
-    rewrite PeanoNat.Nat.add_1_r in H3.
-    apply (PeanoNat.Nat.lt_succ_r l (length s)) in H3.
-    assert (l < length s) by lia.
-    rewrite app_length. simpl. unfold getObj in *.
-    rewrite nth_error_app1 in H1 => //.
-    apply (H _ _ _ H1) in H2. lia.
+  rewrite app_length; simpl.
+  destruct_eq (l = length s);
+    [subst; rewrite_anywhere getObj_last | rewrite_anywhere getObj_last2]; eauto.
+  + invert_constructor_equalities; subst.
+    apply PeanoNat.Nat.lt_trans with (length s); [| lia].
+    eapply H0, nth_error_In, H2.
+  + apply PeanoNat.Nat.lt_trans with (length s); [| lia]; eauto.
+  + apply getObj_dom in H1.
+    rewrite_anywhere  app_length; simpl in *.
+    assert (l < length s) by lia ; eauto.
 Qed.
-Hint Resolve wf_add: wf.
 
 Lemma wf_add_empty : forall s c, wf s -> wf (s ++ [(c,[])]).
 Proof.
   eauto using wf_add, storeSubset_codom_empty.
 Qed.
+
+(** We add all hints *)
+Hint Resolve storeSubset_trans: wf.
+Hint Resolve storeSubset_union: wf.
+Hint Resolve storeSubset_union_l: wf.
+Hint Resolve storeSubset_add: wf.
+Hint Resolve storeSubset_union_r: wf.
+Hint Resolve storeSubset_singleton: wf.
+Hint Resolve storeSubset_singleton2: wf.
+Hint Resolve storeSubset_codom_empty: wf.
+Hint Resolve wf_add: wf.
 Hint Resolve wf_add_empty: wf.
+Hint Resolve nth_error_In: wf.
 
+(** ** Evaluation-maintained results *)
+(** We want to show that the evaluator maintains the wellformedness of stores. As it is not only about stores but also the location of [this] and the result, we cannot use the results proved in Eval.v. We reprove it from scratch, starting with some technical results. *)
 
-Lemma wf_assign: forall σ σ' ω ω' l v f C,
+Lemma wf_assign:
+  forall σ σ' ω ω' l v f C,
     (getObj σ l) = Some (C, ω) ->
     σ' = [l ↦ (C, ω')]σ ->
     ω' = [f ↦ v]ω ->
     v < dom σ ->
     wf σ -> wf σ'.
 Proof.
-  unfold wf; steps. rewrite update_dom.
-  pose proof (PeanoNat.Nat.eq_dec l l0) as [Hl0 | Hl0]; subst.
-  + rewrite getObj_update1 in H4; eauto using getObj_dom.
-    unfold getVal in *.
-    assert (f0 < length ω0). {
-      pose proof (nth_error_Some ω0 f0);
-        destruct (nth_error ω0 f0); eapply_any; steps.
-    }
-    invert_constructor_equalities; subst.
-    pose proof (PeanoNat.Nat.eq_dec f f0) as [Hf | Hf]; subst.
-    ++ rewrite_anywhere update_one3.
-       rewrite update_one1 in H5 => // .
-       invert_constructor_equalities; steps.
-    ++ erewrite update_one2 in H5; eauto.
-  + unfold getObj in *.
-    rewrite update_one2 in H4; eauto using PeanoNat.Nat.neq_sym.
+  unfold wf; steps.
+  rewrite update_dom.
+  getObj_update; steps; eauto.
+  getVal_update; steps; eauto.
 Qed.
 Hint Resolve wf_assign: wf.
 
-
-
-Theorem wellformedness_theorem_list_aux : forall k n ρ ψ,
+(** We have the result for a evaluating a list of arguments *)
+Lemma wellformedness_theorem_list_aux :
+  forall n,
     (forall k : nat,
         k < n ->
-        forall (e : Expr) (σ σ' : Store) (ρ : Env) (ψ l : Value),
-          (⟦ e ⟧ (σ, ρ, ψ )( k)) = Success l σ' -> wf σ -> (codom ρ ∪ {ψ}) ⪽ σ -> wf σ' /\ l < dom σ') ->
-    k < n ->
-    forall el s s' vl1 vl2,
+        forall e σ σ' ρ ψ l,
+          ⟦ e ⟧ (σ, ρ, ψ )( k) = Success l σ' ->
+          wf σ ->
+          (codom ρ ∪ {ψ}) ⪽ σ ->
+          wf σ' /\ l < dom σ') ->
+    forall k, k < n ->
+    forall ρ ψ el s s' vl1 vl2,
       fold_left (eval_list_aux ρ ψ k) el (Success_l vl1 s) = Success_l vl2 s' ->
       wf s ->
       codom vl1 ⪽ s ->
       (codom ρ ∪ {ψ}) ⪽ s ->
       wf s' /\ (codom vl2 ⪽ s') /\ (dom s <= dom s').
 Proof.
-  intros k n ρ ψ H_strong Hn.
+  intros n H_strong k Hn.
   induction el; simpl; intros; try solve [steps].
   destruct k => //; try solve [rewrite foldLeft_constant in H => //].
-  simpl in H.
+  simpl in *; destruct_eval.
+  move: (H3); intros.
+  eapply H_strong in H4 ; eauto with wf; try lia.
+  eapply partialMonotonicity_theorem_dom in H3.
+  eapply IHel in H;
+    steps; try lia;
+       try eapply storeSubset_add;
+      eauto with wf pM.
+Qed.
+
+Ltac update_dom :=
+  repeat rewrite_anywhere update_dom;
+  repeat rewrite update_dom.
+
+Lemma wellformedness_theorem_init_aux:
+  forall n,
+    (forall k : nat,
+        k < n ->
+        forall e σ σ' ρ ψ l,
+          ⟦ e ⟧ (σ, ρ, ψ )( k) = Success l σ' ->
+          wf σ ->
+          (codom ρ ∪ {ψ}) ⪽ σ ->
+          wf σ' /\ l < dom σ') ->
+    forall k, k < n ->
+         forall fields l1 l σ1 σ2,
+           l < dom σ1 ->
+           fold_left (init_field l1 l k) fields (Some σ1) = Some σ2 ->
+           (codom l1 ∪ {l}) ⪽ σ1 ->
+           wf σ1 ->
+           wf σ2 /\ (dom σ1 <= dom σ2).
+Proof.
+  intros n Hstrong k Hn.
+  induction fields; simpl; intros; try solve [steps].
+  destruct k; simpl in H0; try solve [rewrite_anywhere foldLeft_constant  => //].
+  destruct a.
   destruct_eval.
-  apply PeanoNat.Nat.lt_succ_l in Hn.
-  pose proof (H_strong k Hn _ _ _ _ _ _ H3 H0 H2) as [Hwfs2 Hv0].
-  pose proof (PartialMonotonicity.partialMonotonicity_theorem_dom _ _ _ _ _ _ _ H3).
-  assert (codom (v :: vl1) ⪽ s0) by (apply storeSubset_add; eauto using storeSubset_trans).
-  move /(_ _ _ _ _ H Hwfs2 H5 (storeSubset_trans _ s s0 H4 H2)): IHel => IHel.
-  steps; try lia.
+  unfold assign_new in *.
+  destruct_match; try solve [rewrite_anywhere foldLeft_constant  => //].
+  destruct o.
+  eval_dom.
+  eapply Hstrong in H3; eauto with wf; [destruct_and | lia].
+  apply IHfields in H0; clear IHfields;
+    unfold storeSubset; steps; update_dom;
+      eauto with wf lia updates.
+  + destruct_eq (l = l0); subst; eauto with updates lia.
+    induction H6; try inSingleton; steps.
+    eapply storeSubset_union_l in H1.
+    eapply PeanoNat.Nat.le_trans with (dom σ1);
+      eauto with wf lia.
+    eapply H1 => //.
+  + intros l'; intros. update_dom.
+    unfold wf in H3.
+    getObj_update; steps; eauto with wf lia.
+    eapply_anywhere getVal_add; steps; try lia; eauto.
 Qed.
 
 
 Theorem wellformedness_conserved :
-  forall k e σ σ' ρ ψ l,
-    ⟦e⟧(σ, ρ, ψ)(k) = (Success l σ') ->
+  forall n e σ σ' ρ ψ l,
+    ⟦e⟧(σ, ρ, ψ)(n) = (Success l σ') ->
     wf σ ->
     (codom ρ) ∪ {ψ} ⪽ σ ->
     (wf σ' /\ l < dom σ').
 Proof.
-  apply (strong_induction (fun k => forall e σ σ' ρ ψ l, ⟦e⟧(σ, ρ, ψ)(k) = (Success l σ') -> wf σ -> (codom ρ) ∪ {ψ} ⪽ σ ->  (wf σ' /\ l < dom σ'))). intros.
-  assert (ψ < dom σ /\ forall l', List.In l' ρ -> l' < dom σ). {
-    unfold storeSubset in *.
-    split; steps; eauto using Union_introl, Union_intror, In_singleton. }
+  apply (strong_induction (fun k => forall e σ σ' ρ ψ l, ⟦e⟧(σ, ρ, ψ)(k) = (Success l σ') -> wf σ -> (codom ρ) ∪ {ψ} ⪽ σ ->  (wf σ' /\ l < dom σ'))).
+  intros n H_strongInd; intros.
+  assert (ψ < dom σ /\ forall l', List.In l' ρ -> l' < dom σ)
+    by (unfold storeSubset in *;  steps; eauto with wf).
   destruct_and.
   destruct n => //.
   move : (PeanoNat.Nat.lt_succ_diag_r n) => Hn.
-  destruct e ; simpl in H0 ;
-    repeat discriminate || subst || invert_constructor_equalities || destruct_match ||
-           lazymatch goal with
-           | H1 : ⟦ _ ⟧ ( _, _, _)( _ ) = Success _ _ |- _ =>
-             pose proof (PartialMonotonicity.partialMonotonicity_theorem_dom _ _ _ _ _ _ _ H1);
-               pose proof (H n Hn _ _ _ _ _ _ H1); clear H1 end; eauto.
+  destruct e; intros; simpl in *;
+    unfold wf in *;
+      try solve [steps; eauto with wf pM lia];
+      try solve [steps; eapply H_strongInd in matched; steps; eauto with wf pM lia];
+      repeat (destruct_match; try discriminate) || eval_dom.
 
-
-  + intuition auto. eauto using nth_error_In.
-  + intuition auto. unfold wf in *. eapply H6; eauto.
-  + destruct n => //. simpl in *.
-    apply PeanoNat.Nat.lt_succ_l in Hn.
-    pose proof (wellformedness_theorem_list_aux n (S(S n)) ρ ψ H Hn _ _ _ _ _ matched3) as H_list.
-    assert (codom [] ⪽ s) by done.
-    assert ((codom ρ ∪ {ψ}) ⪽ s) by eauto using storeSubset_trans.
-    apply H6; intuition auto.
-    intros l2 Hl2; induction Hl2; eauto.
-    induction H6. lia.
-  + destruct n => //. simpl in *.
-    apply PeanoNat.Nat.lt_succ_l in Hn.
-    pose proof (wellformedness_theorem_list_aux n (S(S n)) ρ ψ H Hn _ _ _ _ _ matched H1 (storeSubset_codom_empty _) H2) as [H_wf_s [H_codom_s H_dom_s]].
-    repeat destruct_match; try discriminate.
-    assert (forall k fields l σ1 σ2,
-               k < S (S n) ->
-               fold_left (init_field l1 l k) fields (Some σ1) = Some σ2 ->
-               (codom l1 ∪ {l}) ⪽ σ1 ->
-               wf σ1 ->
-               wf σ2 /\ (dom σ1 <= dom σ2)). {
-      induction fields0; simpl; intros; try solve [steps].
-      destruct k; simpl in H5; try solve [rewrite_anywhere foldLeft_constant  => //].
-      destruct a.
-      destruct_eval.
-      unfold assign_new in *. destruct_match; try solve [rewrite_anywhere foldLeft_constant  => //].
-      destruct o.
-      pose proof (PartialMonotonicity.partialMonotonicity_theorem_dom _ _ _ _ _ _ _ H8).
-      apply H in H8 => // ; try lia. destruct H8 as [E1 E2].
-      apply IHfields0 in H5; clear IHfields0 => //.
-      ++ steps. unfold dom in *; rewrite_anywhere update_one3. eauto using PeanoNat.Nat.le_trans.
-      ++ apply (storeSubset_trans _ σ1 s0) in H6 => //.
-         apply (storeSubset_trans _ s0) => //.
-         unfold dom in *.
-         rewrite update_one3; eauto.
-      ++ clear H5.
-         intros l'; intros.
-         unfold dom in *. rewrite update_one3.
-         move: (PeanoNat.Nat.eq_dec l l') => [Hl' | Hl'].
-         +++ (* l = l' *)
-           subst.
-           rewrite getObj_update1 in H5; eauto using getObj_dom. invert_constructor_equalities; subst.
-           unfold getVal in *. apply nth_error_Some2 in H8. destruct H8 as [H8 | H8]; subst; eauto.
-         +++ (* l ≠ l' *)
-           unfold getObj in *.
-           rewrite update_one2 in H5 => //. eapply E1; eauto.
-    }
-    apply H0 in matched0; eauto using wf_add_empty.
-    split; steps.
-    unfold dom in *; rewrite_anywhere app_length. simpl in *. lia.
-    apply storeSubset_union. apply (storeSubset_trans _ s _) => //. unfold dom in *; rewrite app_length; lia.
-    unfold storeSubset; intros. induction H5. unfold dom in *; rewrite app_length; simpl ; lia.
-  + unfold assign in *.
-    destruct (getObj s0 v0) eqn:G.
-    ++ destruct o.
-       apply H6. intuition auto.
-       eapply wf_assign; eauto; try eapply H9; eauto using storeSubset_trans.
-       apply (storeSubset_trans _ σ _) => //.
-       unfold dom in *; rewrite update_one3. lia.
-    ++ repeat apply_any; eauto using storeSubset_trans.
+  + destruct n => //.
+    eapply H_strongInd in matched; eauto; destruct_and.
+    eapply wellformedness_theorem_list_aux in matched6;
+      eauto with wf pM lia; try destruct_and.
+    eapply H_strongInd in H; try eapply_any; eauto with wf; destruct_and.
+    eapply storeSubset_union; [| eapply storeSubset_singleton2];
+      eauto with wf lia.
+  + destruct n => //; simpl in *; repeat (destruct_match; try discriminate).
+    eapply wellformedness_theorem_list_aux in matched;
+      eauto with wf pM lia; destruct_and.
+    invert_constructor_equalities; subst.
+    eapply wellformedness_theorem_init_aux in matched0;
+      try rewrite dom_app; try rewrite_anywhere dom_app;
+        eauto with wf lia; try destructs.
+    eapply storeSubset_union; [| eapply storeSubset_singleton2;  rewrite dom_app];
+      eauto with wf lia.
+    intros l Hl; rewrite dom_app.
+    eapply H6 in Hl; eauto with lia.
+  + eapply H_strongInd in matched; eauto; destruct_and.
+    eapply H_strongInd in matched0; eauto with wf;  destruct_and.
+    unfold assign in *.
+    repeat (destruct_match; try discriminate); eauto with wf lia.
+    update_dom.
+    eapply H_strongInd in H ; eauto with wf; try destruct_and.
+    ++ intros.
+       update_dom.
+       getObj_update; steps; eauto.
+       getVal_update; steps; eauto.
+    ++ eapply storeSubset_trans with σ; eauto with wf lia.
+       update_dom; lia.
 Qed.
 Hint Resolve wellformedness_conserved: wf.
 
-
-Theorem wf_conserved :
-  forall k e σ σ' ρ ψ l,
-    ⟦e⟧(σ, ρ, ψ)(k) = (Success l σ') ->
-    wf σ ->
-    (codom ρ) ∪ {ψ} ⪽ σ ->
-    wf σ'.
-Proof.
-  intros. eapply wellformedness_conserved; eauto.
-Qed.
 
 Theorem correct_value :
   forall k e σ σ' ρ ψ l,
@@ -272,8 +298,7 @@ Theorem correct_value :
     (codom ρ) ∪ {ψ} ⪽ σ ->
     l < dom σ'.
 Proof.
-  intros. eapply wellformedness_conserved; eauto.
+  eapply wellformedness_conserved.
 Qed.
 
-Hint Resolve wf_conserved: wf.
 Hint Resolve correct_value: wf.
