Trees.v
@@ -4,9 +4,6 @@ Require Import ssreflect ssrbool.
 Require Import Sets.Ensembles.
 Require Import Celsius.Tactics.
 
-(* Read the pen/paper proofs of scopability *)
-(* Github repo  ? *)
-
 (* Type modifiers *)
 Inductive mode: Set := hot | warm | cold.
 Notation "'@' u " := (u) (at level 20).
@@ -22,24 +19,24 @@ Definition Loc : Type := nat.
 
 (* Expression constructors *)
 Inductive Expr: Type :=
-  | var   : Var -> Expr
-  | this
-  | fld   : Expr -> Var -> Expr
-  | mtd   : Expr -> Mtd -> (list Expr) -> Expr
-  | new   : ClN -> (list Expr) -> Expr
-  | asgn  : Expr -> Var -> Expr -> Expr -> Expr.
+| var   : Var -> Expr
+| this
+| fld   : Expr -> Var -> Expr
+| mtd   : Expr -> Mtd -> (list Expr) -> Expr
+| new   : ClN -> (list Expr) -> Expr
+| asgn  : Expr -> Var -> Expr -> Expr -> Expr.
 
 Inductive Method: Type :=
-  | method(μ: mode)(args: list Tpe)(out_type: Tpe)(body: Expr).
+| method(μ: mode)(args: list Tpe)(out_type: Tpe)(body: Expr).
 
 Inductive Field: Type :=
-  | field(type: Tpe)(expr: Expr).
+| field(type: Tpe)(expr: Expr).
 
 Inductive Class: Type :=
-  | class(args: list Tpe)(fields: list Field)(methods: Mtd -> (option Method)).
+| class(args: list Tpe)(fields: list Field)(methods: Mtd -> (option Method)).
 
 Inductive Program: Type :=
-  | program(C: list Class)(entry: Expr).
+| program(C: list Class)(entry: Expr).
 
 (* Constructs *)
 Definition Value : Type := Loc.
@@ -64,7 +61,7 @@ Definition getVal (l : list Value) := nth_error l.
 Lemma getObj_last : forall (σ: Store) (C: ClN) (ρ: Env), getObj (σ++[(C,ρ)]) (length σ) = Some (C, ρ).
 Proof.
   induction σ; simpl; intros => //.
-  Qed.
+Qed.
 
 Lemma getObj_last2 : forall σ C ρ l, l < dom σ -> getObj (σ++[(C,ρ)]) l = getObj σ l.
 Proof.
@@ -101,8 +98,8 @@ Qed.
 
 Fixpoint removeTypes (l : list (Var*Tpe)) : (list Var) :=
   match l with
-    | [] => []
-    | ((v, t) :: l') => (v::(removeTypes l')) end.
+  | [] => []
+  | ((v, t) :: l') => (v::(removeTypes l')) end.
 
 Fixpoint update_one {X : Type} (position : nat) (value : X)(l : list X) : list X :=
   match (l, position) with
@@ -113,8 +110,8 @@ Fixpoint update_one {X : Type} (position : nat) (value : X)(l : list X) : list X
 
 Fixpoint update_list {X : Type} (positions : list nat) (values : list X) (l : list X) : list X :=
   match (positions, values) with
-    | (x::xt, v::vt) => update_list xt vt (update_one x v l)
-    | (_, _) => l end.
+  | (x::xt, v::vt) => update_list xt vt (update_one x v l)
+  | (_, _) => l end.
 
 Notation "∅" := ([]).
 Notation "[ x ↦ v ] σ" := (update_one x v σ) (at level 0).
@@ -124,147 +121,187 @@ Notation "[ x ⟼ v ] σ" := (update_list x v σ) (at level 0).
 Lemma update_one1 : forall (X: Type) (p: nat) (v: X) (l: list X),
     p < (length l) ->
     (nth_error [p ↦ v]l p) = Some v.
-  Proof.
-    intros X p v.
-    generalize dependent p.
-    induction p.
-    - simpl.
+Proof.
+  intros X p v.
+  generalize dependent p.
+  induction p.
+  - simpl.
     destruct l.
     simpl.
     move :(PeanoNat.Nat.lt_irrefl 0) => h1 => //.
     reflexivity.
-    - destruct l => H.
-      simpl in H.
-      move :(PeanoNat.Nat.nlt_0_r (S p)) => h1 => //.
-      simpl.
-      move :(Lt.lt_S_n p (length l)) => H1.
-      simpl in H.
-      apply H1 in H.
-      apply IHp in H => //.
+  - destruct l => H.
+    simpl in H.
+    move :(PeanoNat.Nat.nlt_0_r (S p)) => h1 => //.
+    simpl.
+    move :(Lt.lt_S_n p (length l)) => H1.
+    simpl in H.
+    apply H1 in H.
+    apply IHp in H => //.
 Qed.
 
 Lemma update_one2 : forall (X: Type) (p p': nat) (v: X) (l: list X),
     p <> p' ->
     (nth_error [p ↦ v]l p') = (nth_error l p').
-  Proof.
-    intros X p.
-    generalize dependent p.
-    induction p; intros; destruct l ; destruct p' => //.
-    - simpl; apply IHp. eauto.
+Proof.
+  intros X p.
+  generalize dependent p.
+  induction p; intros; destruct l ; destruct p' => //.
+  - simpl; apply IHp. eauto.
 Qed.
 
-  Lemma update_one3 : forall (X: Type) (p: nat) (v: X) (l: list X),
-      length ([p ↦ v]l) = length l.
-  Proof.
-    intros X.
-    induction p; intros; destruct l => //.
-    apply (eq_S _ _(IHp _ _ )).
+Lemma update_one3 : forall (X: Type) (p: nat) (v: X) (l: list X),
+    length ([p ↦ v]l) = length l.
+Proof.
+  intros X.
+  induction p; intros; destruct l => //.
+  apply (eq_S _ _(IHp _ _ )).
 Qed.
 
-  Lemma update_dom : forall (σ:Store) p v,
-      dom [p ↦ v]σ = dom σ.
-  Proof.
-    unfold dom; eauto using update_one3.
-  Qed.
+Lemma update_dom : forall (σ:Store) p v,
+    dom [p ↦ v]σ = dom σ.
+Proof.
+  unfold dom; eauto using update_one3.
+Qed.
 
-  Lemma update_one4 : forall (X:Type) (p:nat) (v v': X) l,
-      nth_error [p ↦ v]l p = Some v' -> v = v'.
-  Proof.
-    intros.
-    assert (p < length l). {
-      pose proof (nth_error_Some [p↦v]l p).
-      rewrite update_one3 in H0. apply H0. rewrite H. discriminate.
-    }
-    rewrite update_one1 in H; eauto. injection H => //.
-  Qed.
+Lemma update_one4 : forall (X:Type) (p:nat) (v v': X) l,
+    nth_error [p ↦ v]l p = Some v' -> v = v'.
+Proof.
+  intros.
+  assert (p < length l). {
+    pose proof (nth_error_Some [p↦v]l p).
+    rewrite update_one3 in H0. apply H0. rewrite H. discriminate.
+  }
+  rewrite update_one1 in H; eauto. injection H => //.
+Qed.
 
-  Lemma dom_app: forall σ (C: ClN) (ω: Env), dom (σ ++ ((C, ω)::nil)) = S (dom σ).
-  Proof.
-    intros.
-    unfold dom; rewrite app_length; simpl.
-    Psatz.lia.
-  Qed.
+Lemma dom_app: forall σ (C: ClN) (ω: Env), dom (σ ++ ((C, ω)::nil)) = S (dom σ).
+Proof.
+  intros.
+  unfold dom; rewrite app_length; simpl.
+  Psatz.lia.
+Qed.
+
+Hint Resolve update_one1: updates.
+Hint Resolve update_one2: updates.
+Hint Resolve update_one3: updates.
+Hint Resolve update_one4: updates.
+
+Lemma getVal_update1 :
+  forall ω o x,
+    x < length ω -> (getVal [x ↦ o]ω x) = Some o.
+Proof.
+  unfold getVal; eauto with updates.
+Qed.
+
+Lemma getVal_update2 :
+  forall ω o x x',
+    x < length ω ->
+    x <> x' ->
+    getVal [x ↦ o]ω x' = getVal ω x'.
+Proof.
+  unfold getVal; eauto with updates.
+Qed.
 
 
+Lemma getObj_update1 : forall (σ: Store) (o: Obj) (x: nat),
+    x < dom σ -> (getObj [x ↦ o]σ x) = Some o.
+Proof.
+  unfold getObj; eauto with updates.
+Qed.
 
+Lemma getObj_update2 : forall (σ: Store) (o: Obj) (x x': nat),
+    x < dom σ ->
+    x <> x' ->
+    (getObj [x ↦ o]σ x') = (getObj σ x').
+Proof.
+  unfold getObj; eauto with updates.
+Qed.
 
-  Lemma getObj_update1 : forall (σ: Store) (o: Obj) (x: nat),
-      x < dom σ -> (getObj [x ↦ o]σ x) = Some o.
-  Proof.
-    rewrite /dom /getObj => σ o x.
-    apply : (update_one1 Obj x o σ) => //.
-  Qed.
-
-  Lemma getObj_update2 : forall (σ: Store) (o: Obj) (x x': nat),
-      x < dom σ ->
-      x <> x' ->
-      (getObj [x ↦ o]σ x') = (getObj σ x').
-  Proof.
-    rewrite /dom /getObj => σ o x x'.
-    move : (update_one2 Obj x x' o σ) => //.
-  Qed.
-
-  Lemma getObj_update3: forall σ o o' x x',
-      getObj [x ↦ o]σ x' = Some o' ->
-      x < dom σ ->
-      ((x = x' /\ o = o') \/ (x <> x' /\ (getObj σ x' = Some o'))).
-  Proof.
-    steps;
+Lemma getObj_update3: forall σ o o' x x',
+    getObj [x ↦ o]σ x' = Some o' ->
+    x < dom σ ->
+    ((x = x' /\ o = o') \/ (x <> x' /\ (getObj σ x' = Some o'))).
+Proof.
+  steps;
     destruct (PeanoNat.Nat.eq_dec x x') as [Heq | Hneq]; subst;
-     [ rewrite getObj_update1 in H |
-       rewrite getObj_update2 in H ]; steps.
-  Qed.
+      [ rewrite getObj_update1 in H |
+        rewrite getObj_update2 in H ]; steps.
+Qed.
 
 
-  Lemma getObj_dom : forall (σ: Store) (o: Obj) (l: nat),
-      (getObj σ l) = Some o ->
-      l < (dom σ).
-  Proof.
-    intros σ o.
-    induction σ ; destruct l => //.
-    + move: (PeanoNat.Nat.lt_0_succ (dom σ)) => //.
-    + simpl => H. apply (Lt.lt_n_S _ _ (IHσ _ H)) .
-  Qed.
+Lemma getObj_dom : forall (σ: Store) (o: Obj) (l: nat),
+    (getObj σ l) = Some o ->
+    l < (dom σ).
+Proof.
+  intros σ o.
+  induction σ ; destruct l => //.
+  + move: (PeanoNat.Nat.lt_0_succ (dom σ)) => //.
+  + simpl => H. apply (Lt.lt_n_S _ _ (IHσ _ H)) .
+Qed.
 
-  Lemma nth_error_Some2 : forall {T:Type} e (v:T) f l,
-      nth_error (e ++ [v]) f = Some l ->
-      v = l \/ nth_error e f = Some l.
-  Proof.
-    intros.
-    assert (f < length (e++[v])) by (apply nth_error_Some; rewrite H; discriminate).
-    move: H0; rewrite app_length; simpl; rewrite PeanoNat.Nat.add_1_r => H0.
-    apply Lt.le_lt_or_eq in H0. destruct H0 as [H0 | H0].
-    right. apply Lt.lt_S_n in H0. rewrite nth_error_app1 in H => //.
-    left. injection H0 => H1; subst. rewrite nth_error_app2 in H => //.
-    rewrite <- Minus.minus_diag_reverse in H. simpl in H. injection H => //.
-  Qed.
+Lemma nth_error_Some2 : forall {T:Type} e (v:T) f l,
+    nth_error (e ++ [v]) f = Some l ->
+    v = l \/ nth_error e f = Some l.
+Proof.
+  intros.
+  assert (f < length (e++[v])) by (apply nth_error_Some; rewrite H; discriminate).
+  move: H0; rewrite app_length; simpl; rewrite PeanoNat.Nat.add_1_r => H0.
+  apply Lt.le_lt_or_eq in H0. destruct H0 as [H0 | H0].
+  right. apply Lt.lt_S_n in H0. rewrite nth_error_app1 in H => //.
+  left. injection H0 => H1; subst. rewrite nth_error_app2 in H => //.
+  rewrite <- Minus.minus_diag_reverse in H. simpl in H. injection H => //.
+Qed.
 
-  Lemma getVal_add:
-    forall ω l l' f,
-      getVal (ω ++ [l]) f = Some l' ->
-      (f = length ω /\ l = l') \/ (f < length ω /\ getVal ω f = Some l').
-  Proof.
-    unfold getVal.
-    steps.
-    assert (f < length ω \/ f = length ω) as [Hf | Hf];
-      [
-        apply Lt.le_lt_or_eq, Lt.lt_n_Sm_le;
-        pose proof (nth_error_Some (ω ++ [l]) f) as Hf;
-        rewrite app_length PeanoNat.Nat.add_1_r in Hf;
-        apply Hf
-      | rewrite_anywhere nth_error_app1
-      | rewrite_anywhere nth_error_app2 ] ;
-      steps;
-      rewrite_anywhere PeanoNat.Nat.sub_diag; steps.
-  Qed.
+Lemma getVal_add:
+  forall ω l l' f,
+    getVal (ω ++ [l]) f = Some l' ->
+    (f = length ω /\ l = l') \/ (f < length ω /\ getVal ω f = Some l').
+Proof.
+  unfold getVal.
+  steps.
+  assert (f < length ω \/ f = length ω) as [Hf | Hf];
+    [
+      apply Lt.le_lt_or_eq, Lt.lt_n_Sm_le;
+      pose proof (nth_error_Some (ω ++ [l]) f) as Hf;
+      rewrite app_length PeanoNat.Nat.add_1_r in Hf;
+      apply Hf
+    | rewrite_anywhere nth_error_app1
+    | rewrite_anywhere nth_error_app2 ] ;
+    steps;
+    rewrite_anywhere PeanoNat.Nat.sub_diag; steps.
+Qed.
 
-  Lemma getVal_update:
-    forall ω l l' f f',
-      getVal ([f ↦ l] ω) f' = Some l' ->
-      (f = f' /\ l = l') \/ (f <> f' /\ getVal ω f' = Some l').
-  Proof.
-    unfold getVal; steps.
-    destruct (PeanoNat.Nat.eq_dec f f') as [Heq | Hneq]; subst.
-     + apply update_one4 in H ; steps.
-     + rewrite update_one2 in H; eauto ; steps.
-  Qed.
+Lemma getVal_update:
+  forall ω l l' f f',
+    getVal ([f ↦ l] ω) f' = Some l' ->
+    (f = f' /\ l = l') \/ (f <> f' /\ getVal ω f' = Some l').
+Proof.
+  unfold getVal; steps.
+  destruct (PeanoNat.Nat.eq_dec f f') as [Heq | Hneq]; subst.
+  + apply update_one4 in H ; steps.
+  + rewrite update_one2 in H; eauto ; steps.
+Qed.
+
+Hint Resolve getObj_dom: updates.
+
+
+Ltac getObj_update :=
+  match goal with
+  | H: getObj [?x ↦ ?o] (?σ) ?x' = Some ?o' |- _ => eapply getObj_update3 in H; eauto with updates
+  end.
+Ltac getVal_update :=
+  match goal with
+  | H: getVal [?x ↦ ?o] (?σ) ?x' = Some ?o' |- _ => eapply getVal_update in H; eauto with updates
+  end.
+
+
+Ltac update_dom :=
+  repeat rewrite_anywhere update_dom;
+  repeat rewrite update_dom.
+
+
+Ltac inSingleton :=
+  match goal with
+  |H: ?a ∈ Singleton Loc ?b |- _ => induction H
+  end.
